\(\|u\|^2 + \|v\|^2 + 2 \|u\|\, \|v\| = (\|u\|+\|v\|)^2
\)%%%% Please add \left and \right to all verticals, this is probably a syntactically ambiguous case

\(|u|^2 + |v|^2 + 2 |u|\, |v| = (|u|+|v|)^2
\)%%%% Please add \left and \right to all verticals, this is probably a syntactically ambiguous case

\begin{align*}
\left\|u+v\right\|^2 = \sum_{i=1}^n  (u_i + v_i)^2 &= \sum_{i=1}^n  u_i^2 + \sum_{i=1}^n  v_i^2 + 2\sum_{i=1}^n u_i v_i 
\\&\leq 
\|u\|^2 + \|v\|^2 + 2 \|u\|\, \|v\| = (\|u\|+\|v\|)^2,
\end{align*}%%%% Please add \left and \right to all verticals, this is probably a syntactically ambiguous case
